use proper linked lists

theories/examples/multiset.v
@@ -7,167 +7,210 @@ From iris_ni.proofmode Require Import dwp_tactics.
 From iris_ni.logrel Require Import typemap interp.
 From iris_ni.examples Require Import lock.
 
-Definition cons : val := λ: "hd" "tl", SOME ("hd", "tl").
-Definition nil : val := NONEV.
+(*
+    type node = NONE | SOME int*list
+and type list = ref node
+*)
 
-Definition list_match : val := λ: "ls" "f" "g",
-  match: "ls" with
-    NONE     => "f" #()
+Definition cons : val := λ: "v" "tl",
+   ref (SOME ("v", "tl")).
+Definition nil : expr := ref NONEV.
+
+Definition insert_unordered : val := λ: "hd" "v",
+  "hd" <- SOME ("v", ref !"hd").
+
+Definition insert_loop : val := rec: "loop" "hd" "v" :=
+  match: !"hd" with
+    NONE => "hd" <- SOME ("v", nil)
   | SOME "x" =>
-    let: "hd" := Fst "x" in
+    let: "w" := Fst "x" in
     let: "tl" := Snd "x" in
-    "g" "hd" "tl"
+    if: "w" ≤ "v"
+    then "hd" <- SOME ("v", ref (SOME ("w", "tl")))
+    else "loop" "hd" "v"
   end.
 
-Definition insert_unordered : val := λ: "ls" "v",
-  cons "v" "ls".
-
-Definition insert_ordered : val := rec: "insert" "ls" "v" :=
-  list_match
-    "ls"
-    (λ: <>, cons "v" nil)
-    (λ: "hd" "tl", if: "v" ≤ "hd"
-                   then cons "v" "ls"
-                   else cons "hd" ("insert" "tl" "v")).
+Definition insert_ordered : val := λ: "hd" "v",
+  insert_loop "hd" "v".
 
 Definition insert : val := λ: "l" "v" "f",
   let: "x" := !"l" in
   let: "l-high" := Fst "x" in
   let: "l-low" := Snd "x" in
   if: "f"
-  then "l" <- (insert_unordered "l-high" "v",
-               "l-low")
-  else "l" <- ("l-high",
-               insert_ordered "l-low" "v").
+  then insert_unordered "l-high" "v"
+  else insert_ordered "l-low" "v".
 
-Definition contains_unorderd : val := rec: "contains" "ls" "v" :=
-  list_match
-    "ls"
-    (λ: <>, #false)
-    (λ: "hd" "tl", if: "v" = "hd"
-                   then #true
-                   else "contains" "tl" "v").
-
-Definition contains_ordered : val := rec: "contains" "ls" "v" :=
-  list_match
-    "ls"
-    (λ: <>, #false)
-    (λ: "hd" "tl", if: "v" = "hd"
-                   then #true
-                   else if: "hd" < "v"
-                        then #false
-                        else "contains" "tl" "v").
-
-Definition contains : val := λ: "l" "v",
-  let: "x" := !"l" in
-  let: "l-high" := Fst "x" in
-  let: "l-low" := Snd "x" in
-  if: contains_unorderd "l-high" "v"
-  then #true
-  else contains_ordered "l-low" "v".
-
-Definition size_loop : val := λ: "ls",
-  let: "loop" :=
-     (rec: "loop" "ls" "n" :=
-          list_match
-            "ls"
-            (λ: <>, "n")
-            (λ: "hd" "tl", "loop" "tl" ("n"+#1))) in
-  "loop" "ls" #0.
+Definition size_loop : val := rec: "loop" "hd" "n" :=
+  match: !"hd" with
+    NONE => "n"
+  | SOME "x" =>
+    let: "tl" := Snd "x" in
+    "loop" "tl" ("n"+#1)
+  end.
 
 Definition size : val := λ: "l",
   let: "x" := !"l" in
   let: "l-high" := Fst "x" in
   let: "l-low" := Snd "x" in
-  size_loop "l-low" + size_loop "l-high".
-
-Fixpoint is_list (hd : val) (xs : list val) : Prop :=
-  match xs with
-  | [] => hd = NONEV
-  | x :: xs => ∃ hd', hd = SOMEV (x,hd') ∧ is_list hd' xs
-  end.
-
-(* Two specifications/invariants:
-   1. we can insert arbitrary elements into the list, only length is secure.
-   2. we can insert only low security elements into the list, then lookup is also sequre *)
+  size_loop "l-low" #0 + size_loop "l-high" #0.
 
 Section proof.
   Context `{!heapDG Σ, !typemapG (loc*loc) Σ, !lockG Σ}.
 
-  Definition cell_rel (v1 v2 : val) (ξ : slevel) : iProp Σ :=
-    (∃ (w1 w2 : val) (b : bool),
-        ⌜v1 = (w1, #b)%V⌝ ∗ ⌜v2 = (w2, #b)%V⌝ ∗
-        ⟦ tint (if b then High else Low) ⟧ ξ w1 w2)%I.
+  Program Definition joint_list_pre (P : val -> val -> iProp Σ) :
+    (locC -n> locC -n> iProp Σ) -n> (locC -n> locC -n> iProp Σ)
+    := (λne R hd1 hd2,
+        (hd1 ↦ₗ NONEV ∗ hd2 ↦ᵣ NONEV)
+       ∨ (∃ v1 v2 (tl1 tl2 : loc), hd1 ↦ₗ SOMEV (v1, #tl1) ∗
+                           hd2 ↦ᵣ SOMEV (v2, #tl2) ∗
+                           P v1 v2 ∗
+                           ▷ (R tl1 tl2)))%I.
+  Next Obligation. solve_proper. Qed.
 
-  Definition sec_list hd1 hd2 (l ξ : slevel) :=
-    (∃ xs1 xs2, ⌜is_list hd1 xs1⌝ ∗ ⌜is_list hd2 xs2⌝ ∗
-                 ([∗ list] v1; v2 ∈ xs1;xs2, ⟦ tint l ⟧ ξ v1 v2))%I.
+  Instance joint_list_pre_contractive P : Contractive (joint_list_pre P).
+  Proof. solve_contractive. Qed.
+
+  Definition joint_list P := fixpoint (joint_list_pre P).
+  Lemma joint_list_unfold P hd1 hd2 :
+    joint_list P hd1 hd2 ≡
+       ((hd1 ↦ₗ NONEV ∗ hd2 ↦ᵣ NONEV)
+       ∨ (∃ v1 v2 (tl1 tl2 : loc), hd1 ↦ₗ SOMEV (v1, #tl1) ∗
+                           hd2 ↦ᵣ SOMEV (v2, #tl2) ∗
+                           P v1 v2 ∗
+                           ▷ (joint_list P tl1 tl2)))%I.
+  Proof.
+    rewrite {1}/joint_list.
+    transitivity (joint_list_pre P (fixpoint (joint_list_pre P)) hd1 hd2).
+    { f_equiv. f_equiv. apply fixpoint_unfold. }
+    reflexivity.
+  Qed.
+
+  Definition sec_list (hd1 hd2 : loc) (l ξ : slevel) :=
+    (joint_list (⟦ tint l ⟧ ξ) hd1 hd2)%I.
 
   Definition ls_inv (l1 l2 : loc) (ξ : slevel) :=
-    (∃ hdh1 hdh2 hdl1 hdl2,
-        l1 ↦ₗ (hdh1, hdl1) ∗ l2 ↦ᵣ (hdh2, hdl2) ∗
+    (∃ (hdh1 hdh2 hdl1 hdl2 : loc),
+        l1 ↦ₗ (#hdh1, #hdl1) ∗ l2 ↦ᵣ (#hdh2, #hdl2) ∗
         sec_list hdh1 hdh2 High ξ ∗
         sec_list hdl1 hdl2 Low ξ)%I.
 
-  Lemma insert_low_helper v1 v2 hd1 hd2 xs1 xs2 ξ :
-    ⟦ tint Low ⟧ ξ v1 v2 -∗
-    ([∗ list] v1; v2 ∈ xs1;xs2, ⟦ tint Low ⟧ ξ v1 v2) -∗
-    ⌜is_list hd1 xs1⌝ -∗ ⌜is_list hd2 xs2⌝ -∗
-    DWP insert_ordered hd1 v1 & insert_ordered hd2 v2
-      : λ hd1 hd2, ∃ xs1 xs2, ([∗ list] v1; v2 ∈ xs1;xs2, ⟦ tint Low ⟧ ξ v1 v2) ∗ ⌜is_list hd1 xs1⌝ ∗ ⌜is_list hd2 xs2⌝.
+  Lemma insert_unordered_spec (hd1 hd2 : loc) v1 v2 ξ Φ :
+    ⟦ tint High ⟧ ξ v1 v2 -∗
+    sec_list hd1 hd2 High ξ -∗
+    ▷ (sec_list hd1 hd2 High ξ -∗ Φ #() #()) -∗
+    DWP insert_unordered #hd1 v1
+      & insert_unordered #hd2 v2 : Φ.
   Proof.
-    iIntros "#Hvv Hvs".
-    iLöb as "IH" forall (hd1 hd2 xs1 xs2).
-    iDestruct (big_sepL2_length with "Hvs") as %Hlen.
-    iIntros "#Hr1 #Hr2".
-    iDestruct "Hr1" as %Hxs1. iDestruct "Hr2" as %Hxs2.
-    dwp_rec. dwp_pures. dwp_rec. dwp_pures.
-    destruct xs1 as [|x1 xs1'].
-    - assert (xs2 = []) as ->.
-      { destruct xs2; naive_solver. }
-      rewrite Hxs1 Hxs2.
-      dwp_pures. dwp_rec. dwp_pures.
-      iApply dwp_value. iModIntro.
-      iExists [v1],[v2].
-      iFrame "Hvv Hvs".
-      repeat iSplit; iPureIntro; try naive_solver.
-    - assert (∃ x2 xs2', xs2 = x2::xs2') as [x2 [xs2' ->]].
-      { destruct xs2; naive_solver. }
-      simpl in Hxs1, Hxs2.
-      destruct Hxs1 as [hd1' [-> Hhd1']].
-      destruct Hxs2 as [hd2' [-> Hhd2']].
-      iSimpl in "Hvs". iDestruct "Hvs" as "[H Hvs]".
+    iIntros "#Hvv Hls HΦ".
+    dwp_rec. dwp_pures.
+    dwp_pures. rewrite {1}/sec_list joint_list_unfold.
+    dwp_bind (! _)%E (! _)%E.
+    iDestruct "Hls" as "[[Hhd1 Hhd2]|Hls]".
+    - iApply (heap_lang_lifting.dwp_load with "Hhd1 Hhd2").
+      iNext. iIntros "[Hhd1 Hhd2]".
+
+      dwp_pures. dwp_bind (ref _)%E (ref _)%E.
+      iApply heap_lang_lifting.dwp_alloc.
+      iIntros (nil1 nil2) "Hnil1 Hnil2". iNext.
+
+      dwp_pures. iApply (heap_lang_lifting.dwp_store with "Hhd1 Hhd2").
+      iIntros "Hhd1 Hhd2". iNext.
+
+      iApply "HΦ". rewrite /sec_list.
+      rewrite joint_list_unfold.
+      iRight. iExists _,_,_,_. iFrame "Hhd1 Hhd2 Hvv".
+      iNext. rewrite joint_list_unfold.
+      iLeft; by iFrame.
+    - iDestruct "Hls" as (w1 w2 tl1 tl2) "(Hhd1 & Hhd2 & #Hww & Hls)".
+      iApply (heap_lang_lifting.dwp_load with "Hhd1 Hhd2").
+      iNext. iIntros "[Hhd1 Hhd2]".
+
+      dwp_pures. dwp_bind (ref _)%E (ref _)%E.
+      iApply heap_lang_lifting.dwp_alloc.
+      iIntros (hd1' hd2') "Hhd1' Hhd2'". iNext.
+
+      dwp_pures. iApply (heap_lang_lifting.dwp_store with "Hhd1 Hhd2").
+      iIntros "Hhd1 Hhd2". iNext.
+
+      iApply "HΦ". rewrite /sec_list.
+      rewrite (joint_list_unfold _ hd1 hd2).
+      iRight. iExists _,_,_,_. iFrame "Hhd1 Hhd2 Hvv".
+      iNext. rewrite (joint_list_unfold _ hd1').
+      iRight. iExists _,_,_,_. by iFrame.
+  Qed.
+
+  Lemma insert_ordered_spec (hd1 hd2 : loc) v1 v2 ξ Φ :
+    ⟦ tint Low ⟧ ξ v1 v2 -∗
+    sec_list hd1 hd2 Low ξ -∗
+    ▷ (sec_list hd1 hd2 Low ξ -∗ Φ #() #()) -∗
+    DWP insert_ordered #hd1 v1
+      & insert_ordered #hd2 v2 : Φ.
+  Proof.
+    iIntros "#Hvv Hls HΦ".
+    dwp_rec. dwp_pures.
+    iLöb as "IH" forall (hd1 hd2).
+    dwp_rec. dwp_pures.
+    dwp_bind (! _)%E (! _)%E.
+    rewrite {1}/(sec_list hd1 hd2) joint_list_unfold.
+    iDestruct "Hls" as "[[Hhd1 Hhd2]|Hls]".
+    - iApply (heap_lang_lifting.dwp_load with "Hhd1 Hhd2").
+      iNext. iIntros "[Hhd1 Hhd2]".
+
+      dwp_pures. dwp_bind (ref (InjLV #()))%E (ref (InjLV #()))%E.
+      iApply heap_lang_lifting.dwp_alloc.
+      iIntros (nil1 nil2) "Hnil1 Hnil2". iNext.
+
+      dwp_pures. iApply (heap_lang_lifting.dwp_store with "Hhd1 Hhd2").
+      iIntros "Hhd1 Hhd2". iNext.
+
+      iApply "HΦ". rewrite /sec_list.
+      rewrite joint_list_unfold.
+      iRight. iExists _,_,_,_. iFrame "Hhd1 Hhd2 Hvv".
+      iNext. rewrite joint_list_unfold.
+      iLeft; by iFrame.
+    - iDestruct "Hls" as (w1 w2 tl1 tl2) "(Hhd1 & Hhd2 & #Hww & Hls)".
+      iApply (heap_lang_lifting.dwp_load with "Hhd1 Hhd2").
+      iNext. iIntros "[Hhd1 Hhd2]".
+
       dwp_pures.
-      (* x1 x2, v1 v2 are integers *)
-      iDestruct "H" as (? x -> ->) "H".
-      iDestruct "H" as %Hx.
+
+      (* w1 w2, v1 v2 are integers *)
+      iDestruct "Hww" as (? w -> ->) "H".
+      iDestruct "H" as %Hw.
       assert (Low ⊑ ξ) as Hξ.
       { by destruct ξ. }
-      rewrite (Hx Hξ).
+      rewrite (Hw Hξ).
       iDestruct "Hvv" as (? v -> ->) "H".
       iDestruct "H" as %Hv.
       rewrite (Hv Hξ).
       (* now we can continue symbolic execution *)
+
       dwp_pures. case_bool_decide; dwp_pures.
-      + dwp_rec. dwp_pures.
-        iApply dwp_value.
-        iModIntro. iExists (#v::#x::xs1'),(#v::#x::xs2').
-        iSimpl. iFrame "Hvs". iSplitL.
-        { iSplit; iExists _,_; eauto with iFrame. }
-        iSplit; iPureIntro; naive_solver.
-      + dwp_bind (insert_ordered _ _) (insert_ordered _ _).
-        iApply (dwp_wand with "[Hvs]").
-        { iApply ("IH" with "Hvs"); iPureIntro; done. }
-        clear Hhd1' Hhd2' hd1' hd2' xs1' xs2' Hlen.
-        iIntros (hd1' hd2'). iDestruct 1 as (xs1' xs2') "[Hvs [%%]]".
-        dwp_rec. dwp_pures. iApply dwp_value.
-        iModIntro. iExists (#x::xs1'),(#x::xs2').
-        iSimpl. iFrame. iSplitL.
-        { iExists _,_; eauto with iFrame. }
-        iSplit; iPureIntro; naive_solver.
+      + (* Insert the element here *)
+        dwp_bind (ref _)%E (ref _)%E.
+        iApply heap_lang_lifting.dwp_alloc.
+        iIntros (hd1' hd2') "Hhd1' Hhd2'". iNext.
+
+        dwp_pures. iApply (heap_lang_lifting.dwp_store with "Hhd1 Hhd2").
+        iIntros "Hhd1 Hhd2". iNext.
+
+        iApply "HΦ". rewrite /sec_list.
+        rewrite (joint_list_unfold _ hd1 hd2).
+        iRight. iExists _,_,_,_. iFrame "Hhd1 Hhd2".
+        iSplitR.
+        { iExists _,_. eauto with iFrame. }
+        iNext. rewrite (joint_list_unfold _ hd1' hd2').
+        iRight. iExists _,_,_,_. iFrame "Hhd1' Hhd2' Hls".
+        iExists _,_. eauto with iFrame.
+      + (* Continue with the recursion. *)
+        iApply ("IH" with "[-HΦ] HΦ").
+        rewrite /sec_list (joint_list_unfold _ hd1 hd2).
+        iRight. iExists _,_,_,_. iFrame.
+        iExists _. eauto with iFrame.
   Qed.
 
-  (* Question: can the b's here be different? *)
+  (* TODO: Question: can the b's here be different? *)
   Lemma insert_spec l1 l2 v1 v2 (b : bool) ξ Φ :
     ls_inv l1 l2 ξ -∗
     ⟦ tint (if b then High else Low) ⟧ ξ v1 v2 -∗
@@ -183,71 +226,13 @@ Section proof.
 
     dwp_pures. destruct b; dwp_pures.
     - (* High-security *)
-      dwp_bind (insert_unordered _ v1) (insert_unordered _ v2).
-      dwp_rec. dwp_pures. dwp_rec.
-      dwp_pures. iApply dwp_value.
-      iModIntro. dwp_pures.
-
-      iApply (heap_lang_lifting.dwp_store with "Hl1 Hl2").
-      iIntros "Hl1 Hl2". iNext.
-
-      iApply "HΦ". iExists _,_,_,_. iFrame.
-      rewrite /sec_list.
-      iDestruct "Hhs" as (xs1' xs2' Hxs1' Hxs2') "Hvs".
-      iExists (v1::xs1'), (v2::xs2'). iSimpl. iFrame "Hvs Hvv".
-      iSplit; iPureIntro; naive_solver.
+      iApply (insert_unordered_spec with "Hvv Hhs").
+      iNext. iIntros "Hhs". iApply "HΦ".
+      iExists _,_,_,_. iFrame.
     - (* Low-security *)
-      dwp_bind (insert_ordered _ v1) (insert_ordered _ v2).
-      iApply (dwp_wand with "[Hls]").
-      { iDestruct "Hls" as (hd1 hd2 ??) "Hls".
-        iApply (insert_low_helper with "Hvv Hls [//] [//]"). }
-      iIntros (hdl1' hdl2'). iDestruct 1 as (xs1' xs2') "(Hxs & H1 & H2)".
-      dwp_pures.
-
-      iApply (heap_lang_lifting.dwp_store with "Hl1 Hl2").
-      iIntros "Hl1 Hl2". iNext.
-
-      iApply ("HΦ" with "[-]"). iExists _,_,_,_. iFrame.
-      iExists _,_. iFrame.
-  Qed.
-
-  Lemma size_helper hd1 hd2 l ξ Φ :
-    sec_list hd1 hd2 l ξ -∗
-    (∀ v1 v2, sec_list hd1 hd2 l ξ -∗ ⟦ tint Low ⟧ ξ v1 v2 -∗ Φ v1 v2) -∗
-    DWP size_loop hd1 & size_loop hd2 : Φ.
-  Proof.
-    iIntros "Hls HΦ".
-    iDestruct "Hls" as (xs1 xs2) "Hr".
-    dwp_rec.
-    generalize 0. intros n. dwp_pures.
-    iRevert "Hr". iLöb as "IH" forall (n hd1 hd2 xs1 xs2).
-    iIntros "(Hxs1 & Hxs2 & Hls)".
-    iDestruct (big_sepL2_length with "Hls") as %Hlen.
-    iDestruct "Hxs1" as %Hxs1.
-    iDestruct "Hxs2" as %Hxs2.
-    dwp_rec. dwp_pures.
-    destruct xs1 as [|x1 xs1'].
-    - assert (xs2 = []) as ->.
-      { destruct xs2; naive_solver. }
-      rewrite Hxs1 Hxs2.
-      dwp_pures. iApply dwp_value. iModIntro.
-      iApply ("HΦ" with "[-]").
-      { iExists [],[]. iFrame. iSplit; iPureIntro; naive_solver. }
-      iExists n,n. eauto with iFrame.
-    - assert (∃ x2 xs2', xs2 = x2::xs2') as [x2 [xs2' ->]].
-      { destruct xs2; naive_solver. }
-      simpl in Hxs1, Hxs2.
-      destruct Hxs1 as [hd1' [-> Hhd1']].
-      destruct Hxs2 as [hd2' [-> Hhd2']].
-      dwp_pures.
-      iDestruct "Hls" as "[#Hxx Hls]".
-      iApply ("IH" $! (n+1) with "[HΦ] [-]").
-      { iIntros (v1 v2) "Hhd' Hvv".
-        iApply ("HΦ" with "[-Hvv] Hvv").
-        iDestruct "Hhd'" as (xs1 xs2) "(%&%&?)".
-        iExists (x1::xs1),(x2::xs2). iSimpl.
-        iFrame. iFrame "Hxx". iSplit; iPureIntro; naive_solver. }
-      iFrame "Hls". iSplit; iPureIntro; naive_solver.
+      iApply (insert_ordered_spec with "Hvv Hls").
+      iNext. iIntros "Hls". iApply "HΦ".
+      iExists _,_,_,_. iFrame.
   Qed.
 
   (* TODO: move to logrel/interp.v *)
@@ -270,6 +255,43 @@ Section proof.
     iExists _,_. iPureIntro. naive_solver.
   Qed.
 
+  Lemma size_loop_spec (hd1 hd2 : loc) n1 n2 l ξ Φ :
+    ⟦ tint Low ⟧ ξ n1 n2 -∗
+    sec_list hd1 hd2 l ξ -∗
+    (∀ v1 v2, sec_list hd1 hd2 l ξ -∗ ⟦ tint Low ⟧ ξ v1 v2 -∗ Φ v1 v2) -∗
+    DWP size_loop #hd1 n1 & size_loop #hd2 n2 : Φ.
+  Proof.
+    iIntros "Hns Hls HΦ".
+    iLöb as "IH" forall (n1 n2 hd1 hd2).
+    iDestruct "Hns" as "#Hns". dwp_rec. dwp_pures.
+    dwp_bind (! _)%E (! _)%E.
+    rewrite {1}/(sec_list hd1 hd2) (joint_list_unfold _ hd1 hd2).
+    iDestruct "Hls" as "[[Hhd1 Hhd2]|Hls]".
+    - iApply (heap_lang_lifting.dwp_load with "Hhd1 Hhd2").
+      iNext. iIntros "[Hhd1 Hhd2]".
+
+      dwp_pures. iApply dwp_value.
+      iModIntro. iApply ("HΦ" with "[-Hns] Hns").
+      iClear "IH". rewrite /sec_list joint_list_unfold.
+      iLeft. by iFrame.
+    - iDestruct "Hls" as (w1 w2 tl1 tl2) "(Hhd1 & Hhd2 & #Hww & Hls)".
+      iApply (heap_lang_lifting.dwp_load with "Hhd1 Hhd2").
+      iNext. iIntros "[Hhd1 Hhd2]".
+      dwp_pures.
+
+      dwp_bind (_ + _)%E (_ + _)%E.
+      iApply dwp_wand.
+      { iApply dwp_binop; iApply dwp_value; first by iFrame.
+        iModIntro. iExists _; eauto with iFrame. }
+
+      iIntros (z1 z2) "Hz".
+      iApply ("IH" with "Hz Hls [-]").
+      iClear "IH". iIntros (v1 v2) "Hls Hvv".
+      iApply ("HΦ" with "[-Hvv] Hvv").
+      rewrite /sec_list (joint_list_unfold _ hd1 hd2).
+      iRight. iExists _,_,_,_. by iFrame.
+  Qed.
+
   Lemma size_spec l1 l2 ξ Φ :
     ls_inv l1 l2 ξ -∗
     ▷ (∀ v1 v2, ⟦ tint Low ⟧ ξ v1 v2 -∗ ls_inv l1 l2 ξ -∗ Φ v1 v2) -∗
@@ -281,12 +303,14 @@ Section proof.
     dwp_bind (! _)%E (! _)%E. iApply (dwp_load with "Hl1 Hl2").
     iNext. iIntros "[Hl1 Hl2]".
 
-    dwp_pures. dwp_bind (size_loop _) (size_loop _).
-    iApply (size_helper with "Hhs").
+    dwp_pures. dwp_bind (size_loop _ _) (size_loop _ _).
+    iApply (size_loop_spec with "[] Hhs").
+    { iExists _; eauto with iFrame. }
     iIntros (n1 n2) "Hhs #Hn".
 
-    dwp_bind (size_loop _) (size_loop _).
-    iApply (size_helper with "Hls").
+    dwp_bind (size_loop _ _) (size_loop _ _).
+    iApply (size_loop_spec with "[] Hls").
+    { iExists _; eauto with iFrame. }
     iIntros (m1 m2) "Hls #Hm".
 
     iApply dwp_wand.
